CnfFormula.fst
@@ -1,7 +1,10 @@
 module CnfFormula
 
+// module LP = FStar.List.Tot.Properties
+module L = FStar.List.Tot.Base
+open FStar.Classical
 open Utils
-open FStar.List.Tot.Base
+
 
 
 let valid_literal (lit:int) 
@@ -20,20 +23,21 @@ let lit_to_var (lit:int {valid_literal lit})
 //     : Tot bool (decreases term) 
 //     = match term with
 //         | [] -> true
-//         | hd::tl -> if f hd then verify_validity f tl
+//         | L.hd::L.tl -> if f L.hd then verify_validity f L.tl
 //                     else false
 
 
 let valid_clause (clause : list int)
     // : Tot bool
     // = verify_validity valid_literal clause
-    = forall (lit:int {mem lit clause}) . valid_literal lit
+    = forall (lit:int {L.mem lit clause}) . valid_literal lit
+    // = forall lit . L.mem lit clause ==> valid_literal lit
 
 
 let valid_cnf_formula (f : list (list int))
     // : Tot bool
     // = verify_validity valid_clause f
-    = forall (clause : list int) . mem clause f ==> valid_clause clause
+    = forall (clause : list int) . L.mem clause f ==> valid_clause clause
 
 
 let valid_variable (v:int) 
@@ -42,67 +46,68 @@ let valid_variable (v:int)
 
 
 let variable_in_interval (v:int {valid_variable v}) 
-                         (n:int {0 <= n}) 
-                         (start_interval:int {n <= start_interval}) 
-                         (end_interval:int {start_interval <= end_interval})
+                         (n:nat) 
+                         (start_interval:nat {n <= start_interval}) 
+                         (end_interval:nat {start_interval <= end_interval})
     : Tot bool
     = (0 <= v && v < n) || (start_interval <= v && v < end_interval)
 
 
 let variables_up_to_literal (lit:int {valid_literal lit})
-                            (n:int {n >= 0})
+                            (n:nat)
     : Tot bool
     = 0 <= (lit_to_var lit) && (lit_to_var lit) < n
 
 
 let variables_up_to_clause (clause : list int {valid_clause clause})
-                           (n:int {n >= 0})
+                           (n:nat)
     // : Tot bool (decreases clause)
     // = match clause with
     //     | [] -> true
-    //     | hd::tl -> if variables_up_to_literal hd n then variables_up_to_clause tl n
+    //     | L.hd::L.tl -> if variables_up_to_literal L.hd n then variables_up_to_clause L.tl n
     //                 else false
-    = forall lit . mem lit clause ==> variables_up_to_literal lit n
+    = forall lit . L.mem lit clause ==> variables_up_to_literal lit n
 
 
 let variables_up_to_cnf_formula (rf : list (list int) {valid_cnf_formula rf})
-                                (n:int {n >= 0})
+                                (n:nat)
     // : Tot bool (decreases rf)
     // = match rf with
     //     | [] -> true
-    //     | hd::tl -> if variables_up_to_clause hd n then variables_up_to_cnf_formula tl n
+    //     | L.hd::L.tl -> if variables_up_to_clause L.hd n then variables_up_to_cnf_formula L.tl n
     //                 else false
-    = forall clause . mem clause rf ==> variables_up_to_clause clause n
+    = forall clause . L.mem clause rf ==> variables_up_to_clause clause n
 
 
 let variables_in_interval_literal (lit:int)
-                                  (n:int)
-                                  (start_interval:int)
-                                  (end_interval:int)
-    : Pure bool (requires valid_literal lit && 0 <= n && n <= start_interval && start_interval <= end_interval) 
+                                  (n:nat)
+                                  (start_interval:nat)
+                                  (end_interval:nat)
+    : Pure bool (requires valid_literal lit && n <= start_interval && start_interval <= end_interval) 
                 (ensures fun r -> (r ==> variables_up_to_literal lit end_interval))
     = variable_in_interval (lit_to_var lit) n start_interval end_interval 
 
 
 let rec variables_in_interval_clause (clause : list int)
-                                     (n:int)
-                                     (start_interval:int)
-                                     (end_interval:int)
-    : Pure bool (requires valid_clause clause /\ 0 <= n /\ n <= start_interval /\ start_interval <= end_interval)
-                (ensures fun r -> (r ==> variables_up_to_clause clause end_interval))
+                                     (n:nat)
+                                     (start_interval:nat)
+                                     (end_interval:nat)
+    : Pure bool (requires valid_clause clause /\ n <= start_interval /\ start_interval <= end_interval)
+                (ensures fun r -> (r ==> (variables_up_to_clause clause end_interval /\
+                                          (forall lit . L.mem lit clause ==> variables_in_interval_literal lit n start_interval end_interval))))
     = match clause with
         | [] -> true
         | hd::tl -> if variables_in_interval_literal hd n start_interval end_interval then variables_in_interval_clause tl n start_interval end_interval
                     else false
-    // = forall (lit:int) . mem lit clause ==> variables_in_interval_literal lit n start_interval end_interval
  
 
 let rec variables_in_interval (f : list (list int))
-                              (n:int)
-                              (start_interval:int)
-                              (end_interval:int)
-    : Pure bool (requires valid_cnf_formula f /\ 0 <= n /\ n <= start_interval /\ start_interval <= end_interval)
-                (ensures fun r -> (r ==> variables_up_to_cnf_formula f end_interval))
+                              (n:nat)
+                              (start_interval:nat)
+                              (end_interval:nat)
+    : Pure bool (requires valid_cnf_formula f /\ n <= start_interval /\ start_interval <= end_interval)
+                (ensures fun r -> (r ==> (variables_up_to_cnf_formula f end_interval /\
+                                   (forall clause . L.mem clause f ==> variables_in_interval_clause clause n start_interval end_interval))))
     = match f with 
         | [] -> true
         | hd::tl -> if variables_in_interval_clause hd n start_interval end_interval then variables_in_interval tl n start_interval end_interval
@@ -126,7 +131,7 @@ let max_var_literal (lit:int {valid_literal lit})
 
 let rec max_var_clause (clause : list int)
     : Pure int (requires valid_clause clause)
-               (ensures fun r -> (r >= 0 /\ (forall lit . mem lit clause ==> lit_to_var lit < r) /\ variables_up_to_clause clause r))
+               (ensures fun r -> (r >= 0 /\ (forall lit . L.mem lit clause ==> lit_to_var lit < r) /\ variables_up_to_clause clause r))
     = match clause with
         | [] -> 0
         | hd::tl ->
@@ -136,33 +141,154 @@ let rec max_var_clause (clause : list int)
 
 let rec max_var_cnf_formula (rf : list (list int))
     : Pure int (requires valid_cnf_formula rf)
-               (ensures fun r -> (r >= 0 /\ (forall clause . mem clause rf ==> variables_up_to_clause clause r) /\ variables_up_to_cnf_formula rf r))
+               (ensures fun r -> (r >= 0 /\ (forall clause . L.mem clause rf ==> variables_up_to_clause clause r) /\ variables_up_to_cnf_formula rf r))
     = match rf with
         | [] -> assert (variables_up_to_cnf_formula rf 0); 0
         | hd::tl -> 
         let result = FStar.Math.Lib.max (max_var_clause hd) (max_var_cnf_formula tl) in
-        assert (variables_up_to_clause hd result /\ (forall clause . mem clause tl ==> variables_up_to_clause clause result) /\ variables_up_to_cnf_formula rf result);
+        assert (variables_up_to_clause hd result /\ (forall clause . L.mem clause tl ==> variables_up_to_clause clause result) /\ variables_up_to_cnf_formula rf result);
         result
 
 
+let variables_up_to_max_var_literal (lit:int) (n:nat)
+    : Lemma (requires valid_literal lit && variables_up_to_literal lit n)
+            (ensures n >= max_var_literal lit)
+    = ()
+
+
+let rec variables_up_to_max_var_clause (clause : list int) (n:nat)
+    : Lemma (requires valid_clause clause /\ variables_up_to_clause clause n)
+            (ensures n >= max_var_clause clause)
+    = if L.length clause = 0 then ()
+      else
+      (
+          variables_up_to_max_var_literal (L.hd clause) n;
+          variables_up_to_max_var_clause (L.tl clause) n
+      )
+
+
+let rec variables_up_to_max_var_cnf_formula (rf : list (list int)) (n:nat)
+    : Lemma (requires valid_cnf_formula rf /\ variables_up_to_cnf_formula rf n)
+            (ensures n >= max_var_cnf_formula rf)
+    = if L.length rf = 0 then ()
+      else
+      (
+          variables_up_to_max_var_clause (L.hd rf) n;
+          variables_up_to_max_var_cnf_formula (L.tl rf) n
+      )
+
+
 let truth_value_literal (lit:int {valid_literal lit})
-                        (tau : list bool {variables_up_to_literal lit (length tau)})
+                        (tau : list bool {variables_up_to_literal lit (L.length tau)})
     : bool
-    = if lit < 0 then not (my_nth tau (lit_to_var lit))
-      else my_nth tau (lit_to_var lit)
+    = if lit < 0 then not (L.index tau (lit_to_var lit))
+      else L.index tau (lit_to_var lit)
 
 
 let truth_value_clause (clause : list int {valid_clause clause})
-                       (tau : list bool {variables_up_to_clause clause (length tau)})
-    = exists lit . mem lit clause ==> truth_value_literal lit tau
+                       (tau : list bool {variables_up_to_clause clause (L.length tau)})
+    = exists lit . L.mem lit clause && truth_value_literal lit tau
 
 
 let truth_value_cnf_formula (rf : list (list int) {valid_cnf_formula rf})
-                            (tau : list bool {variables_up_to_cnf_formula rf (length tau)})
-    = forall clause . mem clause rf ==> truth_value_clause clause tau
+                            (tau : list bool {variables_up_to_cnf_formula rf (L.length tau)})
+    = forall clause . L.mem clause rf ==> truth_value_clause clause tau
 
 
-let agree (tau1 : list bool) (tau2 : list bool) (start_interval:nat) 
-          (end_interval:nat {start_interval <= end_interval && length tau1 >= end_interval && length tau2 >= end_interval}) 
-    : bool
-    = interval_of_list tau1 start_interval end_interval = interval_of_list tau2 start_interval end_interval
+// let agree (tau1 : list bool) (tau2 : list bool) (start_interval:nat) 
+//           (end_interval:nat {start_interval <= end_interval && L.length tau1 >= end_interval && L.length tau2 >= end_interval}) 
+//     : bool
+//     = interval_of_list tau1 start_interval end_interval = interval_of_list tau2 start_interval end_interval
+
+
+let negate_literal (v:int) (tau : list bool)
+    : Lemma (requires valid_variable v && L.length tau > v)
+            (ensures truth_value_literal (neg_var_to_lit v) tau = not (truth_value_literal (pos_var_to_lit v) tau))
+    = ()
+
+
+let rec same_list (l1 : list bool) (l2 : list bool) (n:nat)
+    : Lemma (requires L.length l1 = n && L.length l2 = n &&
+                      interval_of_list l1 0 n = interval_of_list l2 0 n)
+            (ensures l1 = l2)
+    = if n = 0 then ()
+      else same_list (L.tl l1) (L.tl l2) (n - 1)
+
+
+// let equal_values (l1 : list bool) (l2 : list bool) (a:nat) (b:nat)
+//     : Lemma (requires a <= b &&
+//                       L.length l1 >= b && L.length l2 >= b &&
+//                       interval_of_list l1 a b = interval_of_list l2 a b)
+//             (ensures forall x . a <= x && x < b ==> L.index l1 x = L.index l2 x)
+//     = ()
+
+
+let rec assignment_relevant_cnf_formula (rf : list (list int)) (tau : list bool) (tau' : list bool) (n:nat)
+    : Lemma (requires valid_cnf_formula rf /\ variables_up_to_cnf_formula rf n /\
+                      L.length tau >= n /\ L.length tau' >= n /\
+                      interval_of_list tau 0 n = interval_of_list tau' 0 n)
+            (ensures truth_value_cnf_formula rf tau == truth_value_cnf_formula rf tau')
+            (decreases %[L.length tau; L.length tau'])
+    = if L.length tau' = n then
+      (
+          if L.length tau = n then 
+          (
+              same_list tau tau' n;
+              assert (tau = tau');
+              ()
+          )
+          else
+          (
+              assert (L.length tau > n);
+              assert (L.length (interval_of_list tau 0 (L.length tau - 1)) >= n);
+              assignment_relevant_cnf_formula rf (interval_of_list tau 0 (L.length tau - 1)) tau' n
+          )
+      )
+      else assignment_relevant_cnf_formula rf tau (interval_of_list tau' 0 (L.length tau' - 1)) n
+
+
+let transfer_truth_value_lit (lit:int) (tau : list bool) (tau' : list bool)
+                             (n:nat) (start_interval:nat) (end_interval:nat)
+    : Lemma (requires valid_literal lit &&
+                      n <= start_interval && start_interval <= end_interval &&
+                      variables_in_interval_literal lit n start_interval end_interval &&
+                      L.length tau >= end_interval && L.length tau' >= end_interval &&
+                      interval_of_list tau 0 n = interval_of_list tau' 0 n &&
+                      interval_of_list tau start_interval end_interval = interval_of_list tau' start_interval end_interval)
+            (ensures truth_value_literal lit tau = truth_value_literal lit tau')
+    = assert ((0 <= lit_to_var lit && lit_to_var lit < n) ||
+             (start_interval <= lit_to_var lit && lit_to_var lit < end_interval));
+      assert (L.index tau (lit_to_var lit) = L.index tau' (lit_to_var lit))
+
+
+let transfer_truth_value_clause (clause : list int) (tau : list bool) (tau' : list bool)
+                                (n:nat) (start_interval:nat) (end_interval:nat)
+    : Lemma (requires valid_clause clause /\
+                      n <= start_interval /\ start_interval <= end_interval /\
+                      variables_in_interval_clause clause n start_interval end_interval /\
+                      L.length tau >= end_interval /\ L.length tau' >= end_interval /\
+                      interval_of_list tau 0 n = interval_of_list tau' 0 n /\
+                      interval_of_list tau start_interval end_interval = interval_of_list tau' start_interval end_interval)
+            (ensures truth_value_clause clause tau == truth_value_clause clause tau')
+    = assert (forall lit . L.mem lit clause ==> (((0 <= lit_to_var lit && lit_to_var lit < n) ||
+                                                (start_interval <= lit_to_var lit && lit_to_var lit < end_interval)) &&
+                                               L.index tau (lit_to_var lit) = L.index tau' (lit_to_var lit)))
+
+
+let transfer_truth_value (rf : list (list int)) (tau : list bool) (tau' : list bool)
+                         (n:nat) (start_interval:nat) (end_interval:nat)
+    : Lemma (requires valid_cnf_formula rf /\
+                      n <= start_interval /\ start_interval <= end_interval /\
+                      variables_in_interval rf n start_interval end_interval /\
+                      L.length tau >= end_interval /\ L.length tau' >= end_interval /\
+                      interval_of_list tau 0 n = interval_of_list tau' 0 n /\
+                      interval_of_list tau start_interval end_interval = interval_of_list tau' start_interval end_interval)
+            (ensures truth_value_cnf_formula rf tau == truth_value_cnf_formula rf tau')
+    = let aux (clause : list int) 
+          : Lemma (requires L.mem clause rf)
+                  (ensures valid_clause clause /\
+                           variables_up_to_clause clause end_interval /\
+                           truth_value_clause clause tau == truth_value_clause clause tau')
+          = transfer_truth_value_clause clause tau tau' n start_interval end_interval
+      in
+      forall_intro (move_requires aux)
