FormulaT.fst
@@ -1,10 +1,13 @@
 module FormulaT
 
-open Utils
+open FStar.List.Tot
 module L = FStar.List.Tot.Base
+module LP = FStar.List.Tot.Properties
 open FStar.Math.Lib
 open FStar.String
 open FStar.Classical
+open Utils
+
 
 
 type formula_t =
@@ -20,7 +23,7 @@ let rec valid_formula_t (f:formula_t)
     : Tot bool (decreases f)
     = match f with
         | Var value -> value >= 0
-        | Not f -> valid_formula_t f
+        | Not f' -> valid_formula_t f'
         | Or f1 f2 -> valid_formula_t f1 && valid_formula_t f2
         | And f1 f2 -> valid_formula_t f1 && valid_formula_t f2
         | Implies f1 f2 -> valid_formula_t f1 && valid_formula_t f2
@@ -31,7 +34,7 @@ let rec variables_up_to (f:formula_t) (n:int)
     : r:bool {r ==> valid_formula_t f}
     = match f with
         | Var value -> 0 <= value && value < n
-        | Not f -> variables_up_to f n
+        | Not f' -> variables_up_to f' n
         | Or f1 f2 -> variables_up_to f1 n && variables_up_to f2 n
         | And f1 f2 -> variables_up_to f1 n && variables_up_to f2 n
         | Implies f1 f2 ->variables_up_to f1 n && variables_up_to f2 n
@@ -42,12 +45,11 @@ let rec variables_up_to_monotone (f:formula_t) (n:int) (n':int)
     : Lemma (requires variables_up_to f n && n <= n')
             (ensures variables_up_to f n')
     = match f with
-        // | Var value -> if 0 <= value && value < n && n <= n' then ()
         | Var value -> ()
-        | Not f -> variables_up_to_monotone f n n'
+        | Not f' -> variables_up_to_monotone f' n n'
         | Or f1 f2 -> variables_up_to_monotone f1 n n'; variables_up_to_monotone f2 n n'
         | And f1 f2 -> variables_up_to_monotone f1 n n'; variables_up_to_monotone f2 n n'
-        | Implies f1 f2 ->variables_up_to_monotone f1 n n'; variables_up_to_monotone f2 n n'
+        | Implies f1 f2 -> variables_up_to_monotone f1 n n'; variables_up_to_monotone f2 n n'
         | DImplies f1 f2 -> variables_up_to_monotone f1 n n'; variables_up_to_monotone f2 n n'
 
 
@@ -56,10 +58,10 @@ let rec max_var (f:formula_t)
                (ensures fun r -> (r >= 0 && variables_up_to f r))
     = match f with
         | Var value -> value + 1
-        | Not f -> 
-            let temp = max_var f in
+        | Not f' -> 
+            let temp = max_var f' in
             let n' = temp in
-            variables_up_to_monotone f temp n';
+            variables_up_to_monotone f' temp n';
             n'
         | Or f1 f2 -> 
             let temp1 = max_var f1 in
@@ -91,12 +93,24 @@ let rec max_var (f:formula_t)
             n'
 
 
+let rec variables_up_to_max_var (f:formula_t) (n:nat)
+    : Lemma (requires variables_up_to f n)
+            (ensures valid_formula_t f && n >= max_var f)
+    = match f with
+        | Var value -> ()
+        | Not f' -> variables_up_to_max_var f' n
+        | Or f1 f2 -> variables_up_to_max_var f1 n; variables_up_to_max_var f2 n
+        | And f1 f2 -> variables_up_to_max_var f1 n; variables_up_to_max_var f2 n
+        | Implies f1 f2 -> variables_up_to_max_var f1 n; variables_up_to_max_var f2 n
+        | DImplies f1 f2 -> variables_up_to_max_var f1 n; variables_up_to_max_var f2 n
+
+
 let rec truth_value (f:formula_t {valid_formula_t f}) 
                     (assignment : list bool {variables_up_to f (L.length assignment)})
     : Tot bool (decreases f)
     = match f with
-        | Var value -> my_nth assignment value
-        | Not f -> not (truth_value f assignment)
+        | Var value -> L.index assignment value
+        | Not f' -> not (truth_value f' assignment)
         | Or f1 f2 -> truth_value f1 assignment || truth_value f2 assignment
         | And f1 f2 -> truth_value f1 assignment && truth_value f2 assignment
         | Implies f1 f2 -> not (truth_value f1 assignment) || truth_value f2 assignment
@@ -111,8 +125,8 @@ let equivalent (f1:formula_t {valid_formula_t f1})
         truth_value f1 tau = truth_value f2 tau
 
 
-let rec seq_false (n:int)
-    : Pure (list bool) (requires n >= 0)
+let rec seq_false (n:nat)
+    : Pure (list bool) (requires True)
                        (ensures fun r -> L.length r = n)
     = if n = 0 then []
       else false::(seq_false (n - 1))
@@ -127,59 +141,67 @@ let rec assignment_relevant (f:formula_t) (n:nat) (tau1 : list bool) (tau2 : lis
                       truth_value f tau1 = truth_value f tau2))
     = match f with
         | Var value -> ()
-        | Not f1 ->
-            assignment_relevant f1 n tau1 tau2;
-            variables_up_to_monotone f1 n (L.length tau1);
-            variables_up_to_monotone f1 n (L.length tau2);
-            assert (truth_value f1 tau1 = truth_value f1 tau2)
+        | Not f' ->
+            variables_up_to_monotone f' n (L.length tau1);
+            variables_up_to_monotone f' n (L.length tau2);
+            assignment_relevant f' n tau1 tau2;
+            assert (truth_value f' tau1 = truth_value f' tau2)
         | Or f1 f2 ->
-            assignment_relevant f1 n tau1 tau2;
-            assignment_relevant f2 n tau1 tau2;
             variables_up_to_monotone f1 n (L.length tau1);
             variables_up_to_monotone f1 n (L.length tau2);
             variables_up_to_monotone f2 n (L.length tau1);
             variables_up_to_monotone f2 n (L.length tau2);
+            assignment_relevant f1 n tau1 tau2;
+            assignment_relevant f2 n tau1 tau2;
             assert (truth_value f1 tau1 = truth_value f1 tau2);
             assert (truth_value f2 tau1 = truth_value f2 tau2)
         | And f1 f2 ->
-            assignment_relevant f1 n tau1 tau2;
-            assignment_relevant f2 n tau1 tau2;
             variables_up_to_monotone f1 n (L.length tau1);
             variables_up_to_monotone f1 n (L.length tau2);
             variables_up_to_monotone f2 n (L.length tau1);
             variables_up_to_monotone f2 n (L.length tau2);
+            assignment_relevant f1 n tau1 tau2;
+            assignment_relevant f2 n tau1 tau2;
             assert (truth_value f1 tau1 = truth_value f1 tau2);
             assert (truth_value f2 tau1 = truth_value f2 tau2)
         | Implies f1 f2 ->
-            assignment_relevant f1 n tau1 tau2;
-            assignment_relevant f2 n tau1 tau2;
             variables_up_to_monotone f1 n (L.length tau1);
             variables_up_to_monotone f1 n (L.length tau2);
             variables_up_to_monotone f2 n (L.length tau1);
             variables_up_to_monotone f2 n (L.length tau2);
+            assignment_relevant f1 n tau1 tau2;
+            assignment_relevant f2 n tau1 tau2;
             assert (truth_value f1 tau1 = truth_value f1 tau2);
             assert (truth_value f2 tau1 = truth_value f2 tau2)
         | DImplies f1 f2 ->
-            assignment_relevant f1 n tau1 tau2;
-            assignment_relevant f2 n tau1 tau2;
             variables_up_to_monotone f1 n (L.length tau1);
             variables_up_to_monotone f1 n (L.length tau2);
             variables_up_to_monotone f2 n (L.length tau1);
             variables_up_to_monotone f2 n (L.length tau2);
+            assignment_relevant f1 n tau1 tau2;
+            assignment_relevant f2 n tau1 tau2;
             assert (truth_value f1 tau1 = truth_value f1 tau2);
             assert (truth_value f2 tau1 = truth_value f2 tau2)
-            
+
 
 let equivalent_trans (f1:formula_t) (f2:formula_t) (f3:formula_t)
-    : Lemma (requires valid_formula_t f1 /\ valid_formula_t f2 /\ valid_formula_t f3 /\ equivalent f1 f2 /\ equivalent f2 f3)
+    : Lemma (requires valid_formula_t f1 /\ valid_formula_t f2 /\ valid_formula_t f3 /\
+                      equivalent f1 f2 /\ equivalent f2 f3)
             (ensures equivalent f1 f3)
     = let aux (tau : list bool) : Lemma (requires variables_up_to f1 (L.length tau) && 
-                                    variables_up_to f3 (L.length tau))
+                                                  variables_up_to f3 (L.length tau))
                                         (ensures truth_value f1 tau = truth_value f3 tau)
           = let temp = seq_false (max_var f2) in 
+            
+            LP.append_length tau temp;
             variables_up_to_monotone f2 (L.length temp) (L.length (L.append tau temp));
+
+            same_values_append [] tau [];
+            same_values_append [] tau temp;
+
             assignment_relevant f1 (L.length tau) tau (L.append tau temp); 
             variables_up_to_monotone f1 (L.length tau) (L.length (L.append tau temp));
+
             assignment_relevant f3 (L.length tau) tau (L.append tau temp);
             variables_up_to_monotone f3 (L.length tau) (L.length (L.append tau temp));
             assert (truth_value f1 tau = truth_value f3 tau)
@@ -190,9 +212,9 @@ let equivalent_trans (f1:formula_t) (f2:formula_t) (f3:formula_t)
 let rec pretty_print (f:formula_t) : Tot string 
     = match f with
         | Var value -> string_of_int value
-        | Not f -> 
-            let f = pretty_print f in 
-            concat "" ["~("; f; ")"]
+        | Not f' -> 
+            let f' = pretty_print f' in 
+            concat "" ["~("; f'; ")"]
         | Or f1 f2 ->  
             let f1 = pretty_print f1 in
             let f2 = pretty_print f2 in
