Tseitin.fst
@@ -1,102 +1,123 @@
 module Tseitin
 
+open FStar.List.Tot
+module L = FStar.List.Tot.Base
+module LP = FStar.List.Tot.Properties
+open FStar.Classical
+open FStar.Ghost
 open FormulaT
 open CnfFormula
 open Utils
 open TseitinCore
-module L = FStar.List.Tot.Base
-open FStar.Classical
+
 
 
 let satisfiable (f:formula_t {valid_formula_t f})
-    = exists tau . L.length tau = max_var f ==> truth_value f tau
+    = exists tau . L.length tau = max_var f && truth_value f tau
 
 
 let satisfiable_cnf_formula (rf : list (list int) {valid_cnf_formula rf})
     = exists tau . L.length tau = max_var_cnf_formula rf ==> truth_value_cnf_formula rf tau
 
 
-let equisatisfiable (f:formula_t {valid_formula_t f}) (rf : list (list int) {valid_cnf_formula rf})
+let equisatisfiable (f:formula_t {valid_formula_t f})
+                    (rf : list (list int) {valid_cnf_formula rf})
     = satisfiable f <==> satisfiable_cnf_formula rf
 
 
-// let rec tseitin_cnf (f:formula_t) (n:nat) (start_interval:nat)
-//     : Pure ((list (list int)) & int & nat)
-//            (requires n <= start_interval)
-//            (ensures fun (rf, v, end_interval) -> (valid f rf v n start_interval end_interval /\
-//                                                   tseitin_same_value f rf v n start_interval end_interval /\
-//                                                   tseitin_can_extend f rf v n start_interval end_interval))
-//     = match f with
-//         | Or f1 f2 ->
-//             let rf1, v1, mid = tseitin_cnf f1 n start_interval in
-//             let rf2, v2, v = tseitin_cnf f2 n mid in
-//             let end_interval = v + 1 in
-//             let rf = L.append (L.append rf1 rf2) (or_clauses v1 v2 v) in
-//             //proveCanExtendOr(f1, rf1, v1, f2, rf2, v2, n, start, mid, v, end, rf);
-//             //proveSameValueOr(f1, rf1, v1, f2, rf2, v2, n, start, mid, v, end, rf);
-//             rf, v, end_interval
-//         | And f1 f2 -> 
-//             let rf1, v1, mid = tseitin_cnf f1 n start_interval in
-//             let rf2, v2, v = tseitin_cnf f2 n mid in
-//             let end_interval = v + 1 in
-//             let rf = L.append (L.append rf1 rf2) (and_clauses v1 v2 v) in
-//             //proveCanExtendAnd(f1, rf1, v1, f2, rf2, v2, n, start, mid, v, end, rf);
-//             //proveSameValueAnd(f1, rf1, v1, f2, rf2, v2, n, start, mid, v, end, rf);
-//             rf, v, end_interval
-//         | Implies f1 f2 ->
-//             let rf1, v1, mid = tseitin_cnf f1 n start_interval in
-//             let rf2, v2, v = tseitin_cnf f2 n mid in
-//             let end_interval = v + 1 in
-//             let rf = L.append (L.append rf1 rf2) (implies_clauses v1 v2 v) in
-//             // proveCanExtendImplies(f1, rf1, v1, f2, rf2, v2, n, start, mid, v, end, rf);
-//             //proveSameValueImplies(f1, rf1, v1, f2, rf2, v2, n, start, mid, v, end, rf);
-//             rf, v, end_interval
-//         | DImplies f1 f2 ->
-//             let rf1, v1, mid = tseitin_cnf f1 n start_interval in
-//             let rf2, v2, v = tseitin_cnf f2 n mid in
-//             let end_interval = v + 1 in
-//             let rf = L.append (L.append rf1 rf2) (dimplies_clauses v1 v2 v) in 
-//             //proveCanExtendDimplies(f1, rf1, v1, f2, rf2, v2, n, start, mid, v, end, rf);
-//             //proveSameValueDimplies(f1, rf1, v1, f2, rf2, v2, n, start, mid, v, end, rf);
-//             rf, v, end_interval
-//         | Not f1 ->
-//             let rf1, v1, v = tseitin_cnf f1 n start_interval in
-//             let end_interval = v + 1 in
-//             let rf = L.append rf1 (not_clauses v1 v) in
-//             // proveCanExtendNot(f1, rf1, v1, n, start, v, end, rf);
-//             //proveSameValueNot(f1, rf1, v1, n, start, v, end, rf);
-//             rf, v, end_interval
-//         | Var value ->
-//             let rf = [] in
-//             let v = value in
-//             let end_interval = start_interval in
-//             let aux (tau : list bool) : Lemma (requires L.length tau = n)
-//                                               (ensures can_extend tau f rf v n start_interval end_interval)
-//                 = let tau' = L.append tau (n_falses (end_interval - n)) in
-//                   assert (L.length tau' = end_interval)
-//                 //   assert (can_extend tau f rf v n start_interval end_interval)
-//             in
-//             forall_intro (move_requires aux);
-//             assert (tseitin_can_extend f rf v n start_interval end_interval);
-//             assert (tseitin_same_value f rf v n start_interval end_interval);
-//             rf, v, end_interval
+let rec tseitin_cnf (f:formula_t) (n:nat) (start_interval:nat)
+    : Pure ((list (list int)) & int & nat)
+           (requires variables_up_to f n && n <= start_interval)
+           (ensures fun (rf, v, end_interval) -> (valid f rf v n start_interval end_interval /\
+                                                  tseitin_same_value f rf v n start_interval end_interval /\
+                                                  tseitin_can_extend f rf v n start_interval end_interval))
+    = match f with
+        | Var value ->
+            let rf = [] in
+            let v = value in
+            let end_interval = start_interval in
+
+            let aux (tau : list bool) : Lemma (requires L.length tau = n)
+                                              (ensures can_extend tau f rf v n start_interval end_interval)
+                = let tau' = tau @ (n_falses (end_interval - n)) in
+                  LP.append_length tau (n_falses (end_interval - n));
+                  assert (L.length tau' = end_interval)
+                //   assert (can_extend tau f rf v n start_interval end_interval)
+            in
+            forall_intro (move_requires aux);
+            assert (tseitin_can_extend f rf v n start_interval end_interval);
+            assert (tseitin_same_value f rf v n start_interval end_interval);
+            rf, v, end_interval
+        | Not f1 ->
+            let rf1, v1, v = tseitin_cnf f1 n start_interval in
+            let end_interval = v + 1 in
+            let rf = L.append rf1 (not_clauses v1 v) in
+            // proveCanExtendNot(f1, rf1, v1, n, start, v, end, rf);
+            //proveSameValueNot(f1, rf1, v1, n, start, v, end, rf);
+            rf, v, end_interval
+        | Or f1 f2 ->
+            let rf1, v1, mid = tseitin_cnf f1 n start_interval in
+            let rf2, v2, v = tseitin_cnf f2 n mid in
+            let end_interval = v + 1 in
+            let rf = L.append (L.append rf1 rf2) (or_clauses v1 v2 v) in
+            //proveCanExtendOr(f1, rf1, v1, f2, rf2, v2, n, start, mid, v, end, rf);
+            //proveSameValueOr(f1, rf1, v1, f2, rf2, v2, n, start, mid, v, end, rf);
+            rf, v, end_interval
+        | And f1 f2 -> 
+            let rf1, v1, mid = tseitin_cnf f1 n start_interval in
+            let rf2, v2, v = tseitin_cnf f2 n mid in
+            let end_interval = v + 1 in
+            let rf = L.append (L.append rf1 rf2) (and_clauses v1 v2 v) in
+            //proveCanExtendAnd(f1, rf1, v1, f2, rf2, v2, n, start, mid, v, end, rf);
+            //proveSameValueAnd(f1, rf1, v1, f2, rf2, v2, n, start, mid, v, end, rf);
+            rf, v, end_interval
+        | Implies f1 f2 ->
+            let rf1, v1, mid = tseitin_cnf f1 n start_interval in
+            let rf2, v2, v = tseitin_cnf f2 n mid in
+            let end_interval = v + 1 in
+            let rf = L.append (L.append rf1 rf2) (implies_clauses v1 v2 v) in
+            // proveCanExtendImplies(f1, rf1, v1, f2, rf2, v2, n, start, mid, v, end, rf);
+            //proveSameValueImplies(f1, rf1, v1, f2, rf2, v2, n, start, mid, v, end, rf);
+            rf, v, end_interval
+        | DImplies f1 f2 ->
+            let rf1, v1, mid = tseitin_cnf f1 n start_interval in
+            let rf2, v2, v = tseitin_cnf f2 n mid in
+            let end_interval = v + 1 in
+            let rf = L.append (L.append rf1 rf2) (dimplies_clauses v1 v2 v) in 
+            //proveCanExtendDimplies(f1, rf1, v1, f2, rf2, v2, n, start, mid, v, end, rf);
+            //proveSameValueDimplies(f1, rf1, v1, f2, rf2, v2, n, start, mid, v, end, rf);
+            rf, v, end_interval
+
+
+let satisfied_formula (f:formula_t) (tau : list bool)
+    : Lemma (requires valid_formula_t f && variables_up_to f (L.length tau))
+            (ensures satisfiable f)
+    = let n : erased nat = max_var f in
+      assert (variables_up_to f n);
+      variables_up_to_max_var f (L.length tau);
+      let tau' : erased (list bool) = interval_of_list tau 0 n in
+      assignment_relevant f n tau tau'
+
+
+let satisfied_cnf_formula (rf : list (list int)) (tau : list bool)
+    : Lemma (requires valid_cnf_formula rf /\ 
+                      variables_up_to_cnf_formula rf (L.length tau) /\
+                      truth_value_cnf_formula rf tau)
+            (ensures satisfiable_cnf_formula rf)
+    = let n : erased nat = max_var_cnf_formula rf in
+      assert (variables_up_to_cnf_formula rf n);
+      variables_up_to_max_var_cnf_formula rf (L.length tau);
+      assert (L.length tau >= n);
+      let tau' : erased (list bool) = interval_of_list tau 0 n in
+      assignment_relevant_cnf_formula rf tau tau' n
+
 
 // let tseitin (f:formula_t)
 //     : Pure (list (list int)) (requires valid_formula_t f)
 //                              (ensures fun r -> (valid_cnf_formula r /\ equisatisfiable f r))
 //     = let n = max_var f in
+//       let rf, v, end_interval = tseitin_cnf f n n in
+//       let r = L.append rf [[pos_var_to_lit v]] in
+//       //tseitin_follows f rf v n end_interval;
+//       r
 
-
-//  method tseitin(f : FormulaT) returns (result : seq<seq<int>>)
-//         requires validFormulaT(f);
-//         ensures validCnfFormula(result);
-//         ensures equiSatisfiable(f, result);
-//     {
-//         var n := maxVar(f);
-//         var v : int;
-//         var end : int;
-//         var rf : seq<seq<int>>;
-//         rf, v, end := tseitinCnf(f, n, n);
-//         result := rf + [[posVarToLit(v)]];
-//         tseitinFollows(f, rf, v, n, end);
-//     }
