TseitinCore.fst
@@ -1,9 +1,12 @@
 module TseitinCore
 
+open FStar.List.Tot
 module L = FStar.List.Tot.Base
+module LP = FStar.List.Tot.Properties
 open FormulaT
 open CnfFormula
 open Utils
+
 
 
 let extend (tau : list bool) (tau' : list bool) (n:nat) (start_interval:nat) (end_interval:nat)
@@ -12,10 +15,17 @@ let extend (tau : list bool) (tau' : list bool) (n:nat) (start_interval:nat) (en
                                  L.length tau = n && 
                                  L.length tau' = end_interval - start_interval)
                        (ensures fun r -> (L.length r = end_interval && 
-                                          agree r tau 0 n && 
+                                          interval_of_list r 0 n = tau &&
                                           interval_of_list r start_interval end_interval = tau'))
-    = let up_to_start = L.append tau (n_falses (start_interval - n)) in
-      L.append up_to_start tau'
+    = let falses = n_falses (start_interval - n) in
+      let r = tau @ falses @ tau' in 
+      LP.append_assoc tau falses tau';
+      LP.append_length tau falses;
+      LP.append_length (tau @ falses) tau';
+      same_values_append [] tau (falses @ tau');
+      assert (interval_of_list r 0 n = tau);
+      same_values_append (tau @ falses) tau' [];
+      r
 
 
 let valid (f:formula_t) (rf : list (list int)) (v:int) (n:nat) (start_interval:nat) (end_interval:nat)
@@ -42,28 +52,35 @@ let tseitin_can_extend (f:formula_t) (rf : list (list int)) (v:int) (n:nat) (sta
     = forall (tau : list bool) . L.length tau = n ==> can_extend tau f rf v n start_interval end_interval
 
 
-let and_clauses (v1:int {valid_variable v1}) 
-                (v2:int {valid_variable v2}) 
-                (v:int {valid_variable v}) 
-    : list (list int)
-    = [[neg_var_to_lit v; pos_var_to_lit v1];
-       [neg_var_to_lit v; pos_var_to_lit v2];
-       [neg_var_to_lit v1; neg_var_to_lit v2; pos_var_to_lit v]]
+let not_clauses (v1:int {valid_variable v1})
+                (v:int {valid_variable v})
+    : r : list (list int) {valid_cnf_formula r}
+    = [[neg_var_to_lit v; neg_var_to_lit v1];
+       [pos_var_to_lit v1; pos_var_to_lit v]]
 
 
 let or_clauses (v1:int {valid_variable v1}) 
                (v2:int {valid_variable v2}) 
                (v:int {valid_variable v}) 
-    : list (list int)
+    : r : list (list int) {valid_cnf_formula r}
     = [[neg_var_to_lit v; pos_var_to_lit v1; pos_var_to_lit v2];
        [neg_var_to_lit v1; pos_var_to_lit v];
        [neg_var_to_lit v2; pos_var_to_lit v]]
 
 
+let and_clauses (v1:int {valid_variable v1}) 
+                (v2:int {valid_variable v2}) 
+                (v:int {valid_variable v}) 
+    : r : list (list int) {valid_cnf_formula r}
+    = [[neg_var_to_lit v; pos_var_to_lit v1];
+       [neg_var_to_lit v; pos_var_to_lit v2];
+       [neg_var_to_lit v1; neg_var_to_lit v2; pos_var_to_lit v]]
+
+
 let implies_clauses (v1:int {valid_variable v1}) 
                     (v2:int {valid_variable v2}) 
                     (v:int {valid_variable v}) 
-    : list (list int)
+    : r : list (list int) {valid_cnf_formula r}
     = [[neg_var_to_lit v; neg_var_to_lit v1; pos_var_to_lit v2];
        [pos_var_to_lit v1; pos_var_to_lit v];
        [neg_var_to_lit v2; pos_var_to_lit v]]
@@ -72,18 +89,11 @@ let implies_clauses (v1:int {valid_variable v1})
 let dimplies_clauses (v1:int {valid_variable v1}) 
                      (v2:int {valid_variable v2}) 
                      (v:int {valid_variable v}) 
-    : list (list int)
+    : r : list (list int) {valid_cnf_formula r}
     = [[neg_var_to_lit v; neg_var_to_lit v1; pos_var_to_lit v2];
-       [neg_var_to_lit v1; neg_var_to_lit v1; pos_var_to_lit v];
+       [neg_var_to_lit v1; neg_var_to_lit v2; pos_var_to_lit v];
        [pos_var_to_lit v1; pos_var_to_lit v2; pos_var_to_lit v];
        [neg_var_to_lit v; neg_var_to_lit v2; pos_var_to_lit v1]]
-
-
-let not_clauses (v1:int {valid_variable v1})
-                (v:int {valid_variable v})
-    : list (list int)
-    = [[neg_var_to_lit v; neg_var_to_lit v1];
-       [pos_var_to_lit v1; pos_var_to_lit v]]
 
 
 let combine (tau : list bool) (tau1 : list bool) (tau2 : list bool) (n:nat) 
@@ -91,12 +101,45 @@ let combine (tau : list bool) (tau1 : list bool) (tau2 : list bool) (n:nat)
     : Pure (list bool) (requires n <= start_interval && start_interval <= mid && mid <= end_interval &&
                                  L.length tau = n && L.length tau1 = mid && L.length tau2 = end_interval)
                        (ensures fun r -> (L.length r = end_interval + 1 &&
-                                          agree r tau 0 n &&
-                                          agree r tau1 start_interval mid &&
-                                          agree r tau2 mid end_interval &&
-                                          my_nth r (L.length r - 1) = last))
-    = L.append (L.append (L.append (L.append tau (n_falses (start_interval - n))) 
-    (interval_of_list tau1 start_interval mid)) (interval_of_list tau2 mid end_interval)) [last]
+                                          interval_of_list r 0 n = tau &&
+                                          interval_of_list r start_interval mid = interval_of_list tau1 start_interval mid &&
+                                          interval_of_list r mid end_interval = interval_of_list tau2 mid end_interval && 
+                                          interval_of_list r end_interval (end_interval + 1) = [last]))
+    = let falses = n_falses (start_interval - n) in
+      let from_tau1 = interval_of_list tau1 start_interval mid in
+      let from_tau2 = interval_of_list tau2 mid end_interval in
+      let l1 = tau @ falses in
+      let l2 = l1 @ from_tau1 in
+      let l3 = l2 @ from_tau2 in
+      let r = l3 @ [last] in
+
+      LP.append_assoc tau falses from_tau1;
+      LP.append_assoc tau falses (from_tau1 @ from_tau2);
+      LP.append_assoc tau falses (from_tau1 @ from_tau2 @ [last]);
+
+      LP.append_assoc l1 from_tau1 from_tau2;
+      LP.append_assoc l1 from_tau1 (from_tau2 @ [last]);
+
+      LP.append_assoc l2 from_tau2 [last];
+
+      LP.append_length tau falses;
+      LP.append_length l1 from_tau1;
+      LP.append_length l2 from_tau2;
+      LP.append_length l3 [last];
+
+      assert (r = [] @ tau @ (falses @ from_tau1 @ from_tau2 @ [last]));
+      same_values_append [] tau (falses @ from_tau1 @ from_tau2 @ [last]);
+
+      assert (r = l1 @ from_tau1 @ (from_tau2 @ [last]));
+      same_values_append l1 from_tau1 (from_tau2 @ [last]);
+
+      assert (r = l2 @ from_tau2 @ [last]);
+      same_values_append l2 from_tau2 [last];
+
+      assert (r = l3 @ [last] @ []);
+      same_values_append l3 [last] [];
+
+      r
 
 
 let combine1 (tau : list bool) (tau1 : list bool) (n:nat) (start_interval:nat)
@@ -105,11 +148,35 @@ let combine1 (tau : list bool) (tau1 : list bool) (n:nat) (start_interval:nat)
                                  start_interval <= v &&
                                  L.length tau = n &&
                                  L.length tau1 = v)
-                       (ensures fun r -> (L.length r = v + 1 /\
-                                          agree r tau 0 n /\
-                                          agree r tau1 start_interval v))
-    = L.append (L.append (L.append tau (n_falses (start_interval - n))) (interval_of_list tau1 start_interval v)) [last]
-   
+                       (ensures fun r -> (L.length r = v + 1 &&
+                                          interval_of_list r 0 n = tau &&
+                                          interval_of_list r start_interval v = interval_of_list tau1 start_interval v &&
+                                          interval_of_list r v (v + 1) = [last]))
+    = let falses =  n_falses (start_interval - n) in
+      let from_tau1 = interval_of_list tau1 start_interval v in
+      let l1 = tau @ falses in
+      let l2 = l1 @ from_tau1 in
+      let r = l2 @ [last] in
+
+      LP.append_assoc tau falses from_tau1;
+      LP.append_assoc tau falses (from_tau1 @ [last]);
+      LP.append_assoc l1 from_tau1 [last];
+
+      LP.append_length tau falses;
+      LP.append_length l1 from_tau1;
+      LP.append_length l2 [last];
+
+      assert (r = [] @ tau @ (falses @ from_tau1 @ [last]));
+      same_values_append [] tau (falses @ from_tau1 @ [last]);
+
+      assert (r = l1 @ from_tau1 @ [last]);
+      same_values_append l1 from_tau1 [last];
+
+      assert (r = l2 @ [last] @ []);
+      same_values_append l2 [last] [];
+
+      r
+
 
 let tseitin_same_value (f:formula_t) (rf : list (list int)) (v:int) (n:nat) (start_interval:nat)
                        (end_interval:nat {valid f rf v n start_interval end_interval})
@@ -123,14 +190,123 @@ let tseitin_same_value (f:formula_t) (rf : list (list int)) (v:int) (n:nat) (sta
 let lemma_not_clauses (v1:int) (v:int) (tau : list bool)
     : Lemma (requires valid_variable v1 && valid_variable v && L.length tau > v && L.length tau > v1)
             (ensures truth_value_cnf_formula (not_clauses v1 v) tau <==> 
-            ((not (truth_value_literal (pos_var_to_lit v1) tau)) <==> truth_value_literal (pos_var_to_lit v) tau))
+               ((not (truth_value_literal (pos_var_to_lit v1) tau)) <==> 
+               truth_value_literal (pos_var_to_lit v) tau))
     = let rf = not_clauses v1 v in
       assert (truth_value_cnf_formula rf tau <==> 
-                truth_value_clause (my_nth rf 0) tau /\
-                truth_value_clause (my_nth rf 1) tau);
-      assert (truth_value_clause (my_nth rf 0) tau <==>
-                truth_value_literal (my_nth (my_nth rf 0) 0) tau ||
-                truth_value_literal (my_nth (my_nth rf 0) 1) tau);
-      assert (truth_value_clause (my_nth rf 1) tau <==>
-                truth_value_literal (my_nth (my_nth rf 1) 0) tau ||
-                truth_value_literal (my_nth (my_nth rf 1) 1) tau)
+                truth_value_clause (L.index rf 0) tau /\
+                truth_value_clause (L.index rf 1) tau);
+      assert (truth_value_clause (L.index rf 0) tau <==>
+                truth_value_literal (L.index (L.index rf 0) 0) tau ||
+                truth_value_literal (L.index (L.index rf 0) 1) tau);
+      assert (truth_value_clause (L.index rf 1) tau <==>
+                truth_value_literal (L.index (L.index rf 1) 0) tau ||
+                truth_value_literal (L.index (L.index rf 1) 1) tau)
+
+
+let lemma_or_clauses (v1:int) (v2:int) (v:int) (tau : list bool)
+    : Lemma (requires valid_variable v1 && valid_variable v2 && valid_variable v &&
+                      L.length tau > v1 && L.length tau > v2 && L.length tau > v)
+            (ensures variables_up_to_cnf_formula (or_clauses v1 v2 v) (L.length tau) /\
+                     truth_value_cnf_formula (or_clauses v1 v2 v) tau <==>
+                  ((truth_value_literal (pos_var_to_lit v1) tau || 
+                  truth_value_literal (pos_var_to_lit v2) tau) <==>
+                  truth_value_literal (pos_var_to_lit v) tau))
+    = let rf = or_clauses v1 v2 v in
+      assert (truth_value_cnf_formula rf tau <==>
+                truth_value_clause (L.index rf 0) tau /\
+                truth_value_clause (L.index rf 1) tau /\
+                truth_value_clause (L.index rf 2) tau);
+      assert (truth_value_clause (L.index rf 0) tau <==>
+                truth_value_literal (L.index (L.index rf 0) 0) tau ||
+                truth_value_literal (L.index (L.index rf 0) 1) tau ||
+                truth_value_literal (L.index (L.index rf 0) 2) tau);
+      assert (truth_value_clause (L.index rf 1) tau <==>
+                truth_value_literal (L.index (L.index rf 1) 0) tau ||
+                truth_value_literal (L.index (L.index rf 1) 1) tau);
+      assert (truth_value_clause (L.index rf 2) tau <==>
+                truth_value_literal (L.index (L.index rf 2) 0) tau ||
+                truth_value_literal (L.index (L.index rf 2) 1) tau)
+                  
+
+let lemma_and_clauses (v1:int) (v2:int) (v:int) (tau : list bool)
+    : Lemma (requires valid_variable v1 && valid_variable v2 && valid_variable v &&
+                      L.length tau > v1 && L.length tau > v2 && L.length tau > v)
+            (ensures variables_up_to_cnf_formula (and_clauses v1 v2 v) (L.length tau) /\
+                     truth_value_cnf_formula (and_clauses v1 v2 v) tau <==>
+                  ((truth_value_literal (pos_var_to_lit v1) tau && 
+                  truth_value_literal (pos_var_to_lit v2) tau) <==>
+                  truth_value_literal (pos_var_to_lit v) tau))
+    = let rf = and_clauses v1 v2 v in
+      assert (truth_value_cnf_formula rf tau <==>
+                truth_value_clause (L.index rf 0) tau /\
+                truth_value_clause (L.index rf 1) tau /\
+                truth_value_clause (L.index rf 2) tau);
+      assert (truth_value_clause (L.index rf 0) tau <==>
+                truth_value_literal (L.index (L.index rf 0) 0) tau ||
+                truth_value_literal (L.index (L.index rf 0) 1) tau);
+      assert (truth_value_clause (L.index rf 1) tau <==>
+                truth_value_literal (L.index (L.index rf 1) 0) tau ||
+                truth_value_literal (L.index (L.index rf 1) 1) tau);
+      assert (truth_value_clause (L.index rf 2) tau <==>
+                truth_value_literal (L.index (L.index rf 2) 0) tau ||
+                truth_value_literal (L.index (L.index rf 2) 1) tau ||
+                truth_value_literal (L.index (L.index rf 2) 2) tau)
+        
+
+let lemma_implies_clauses (v1:int) (v2:int) (v:int) (tau : list bool)
+    : Lemma (requires valid_variable v1 && valid_variable v2 && valid_variable v &&
+                      L.length tau > v1 && L.length tau > v2 && L.length tau > v)
+            (ensures variables_up_to_cnf_formula (implies_clauses v1 v2 v) (L.length tau) /\
+                     truth_value_cnf_formula (implies_clauses v1 v2 v) tau <==>
+                  ((truth_value_literal (pos_var_to_lit v1) tau ==> 
+                  truth_value_literal (pos_var_to_lit v2) tau) <==>
+                  truth_value_literal (pos_var_to_lit v) tau))
+    = let rf = implies_clauses v1 v2 v in
+      assert (truth_value_cnf_formula rf tau <==>
+                truth_value_clause (L.index rf 0) tau /\
+                truth_value_clause (L.index rf 1) tau /\
+                truth_value_clause (L.index rf 2) tau);
+      assert (truth_value_clause (L.index rf 0) tau <==>
+                truth_value_literal (L.index (L.index rf 0) 0) tau ||
+                truth_value_literal (L.index (L.index rf 0) 1) tau ||
+                truth_value_literal (L.index (L.index rf 0) 2) tau);
+      assert (truth_value_clause (L.index rf 1) tau <==>
+                truth_value_literal (L.index (L.index rf 1) 0) tau ||
+                truth_value_literal (L.index (L.index rf 1) 1) tau);
+      assert (truth_value_clause (L.index rf 2) tau <==>
+                truth_value_literal (L.index (L.index rf 2) 0) tau ||
+                truth_value_literal (L.index (L.index rf 2) 1) tau)
+
+
+let lemma_dimplies_clauses (v1:int) (v2:int) (v:int) (tau : list bool)
+    : Lemma (requires valid_variable v1 && valid_variable v2 && valid_variable v &&
+                      L.length tau > v1 && L.length tau > v2 && L.length tau > v)
+            (ensures variables_up_to_cnf_formula (dimplies_clauses v1 v2 v) (L.length tau) /\
+                     truth_value_cnf_formula (dimplies_clauses v1 v2 v) tau <==>
+                  ((truth_value_literal (pos_var_to_lit v1) tau <==> 
+                  truth_value_literal (pos_var_to_lit v2) tau) <==>
+                  truth_value_literal (pos_var_to_lit v) tau))
+    = let rf = dimplies_clauses v1 v2 v in
+      //assert (variables_up_to_cnf_formula rf (L.length tau));
+      assert (truth_value_cnf_formula rf tau <==>
+                truth_value_clause (L.index rf 0) tau /\
+                truth_value_clause (L.index rf 1) tau /\
+                truth_value_clause (L.index rf 2) tau /\
+                truth_value_clause (L.index rf 3) tau );
+      assert (truth_value_clause (L.index rf 0) tau <==>
+                truth_value_literal (L.index (L.index rf 0) 0) tau ||
+                truth_value_literal (L.index (L.index rf 0) 1) tau ||
+                truth_value_literal (L.index (L.index rf 0) 2) tau);
+      assert (truth_value_clause (L.index rf 1) tau <==>
+                truth_value_literal (L.index (L.index rf 1) 0) tau ||
+                truth_value_literal (L.index (L.index rf 1) 1) tau ||
+                truth_value_literal (L.index (L.index rf 1) 2) tau);
+      assert (truth_value_clause (L.index rf 2) tau <==>
+                truth_value_literal (L.index (L.index rf 2) 0) tau ||
+                truth_value_literal (L.index (L.index rf 2) 1) tau ||
+                truth_value_literal (L.index (L.index rf 2) 2) tau);
+      assert (truth_value_clause (L.index rf 3) tau <==>
+                truth_value_literal (L.index (L.index rf 3) 0) tau ||
+                truth_value_literal (L.index (L.index rf 3) 1) tau ||
+                truth_value_literal (L.index (L.index rf 3) 2) tau)
