TseitinProofs.fst
@@ -1,11 +1,22 @@
 module TseitinProofs
 
+open FStar.List.Tot
+module L = FStar.List.Tot.Base
+module LP = FStar.List.Tot.Properties
+open FStar.Classical
+open FStar.Ghost
 open CnfFormula
 open FormulaT
 open Utils
 open TseitinCore
-module L = FStar.List.Tot.Base
-open FStar.Classical
+
+
+
+let rec append_valid_cnf_formulas (f1 : list (list int)) (f2 : list (list int))
+    : Lemma (requires valid_cnf_formula f1 /\ valid_cnf_formula f2)
+            (ensures valid_cnf_formula (f1 @ f2))
+    = if L.length f1 = 0 then ()
+      else append_valid_cnf_formulas (tl f1) f2
 
 
 let prove_same_value_not (f1:formula_t) (rf1 : list (list int)) (v1:int) (n:nat)
@@ -13,80 +24,184 @@ let prove_same_value_not (f1:formula_t) (rf1 : list (list int)) (v1:int) (n:nat)
     : Lemma (requires n <= start_interval /\ start_interval <= v /\
                       valid f1 rf1 v1 n start_interval v /\
                       tseitin_same_value f1 rf1 v1 n start_interval v /\
-                      rf = L.append rf1 (not_clauses v1 v) /\ end_interval = v + 1)
+                      rf = rf1 @ (not_clauses v1 v) /\
+                      end_interval = v + 1)
             (ensures valid (Not f1) rf v n start_interval end_interval /\
                      tseitin_same_value (Not f1) rf v n start_interval end_interval)
-    = assert (valid (Not f1) rf v n start_interval end_interval);
-      let aux (tau : list bool) : Lemma (requires L.length tau >= end_interval /\
-                                                  truth_value_cnf_formula rf tau)
-                                        (ensures truth_value_literal (pos_var_to_lit v) tau = truth_value (Not f1) tau)
+    = append_valid_cnf_formulas rf1 (not_clauses v1 v);
+
+
+      assert (variables_in_interval rf n start_interval end_interval);
+      // assert (valid (Not f1) rf v n start_interval end_interval);
+
+      let aux (tau : list bool) 
+          : Lemma (requires L.length tau >= end_interval /\
+                            truth_value_cnf_formula rf tau)
+                  (ensures truth_value_literal (pos_var_to_lit v) tau = truth_value (Not f1) tau)
           = variables_up_to_monotone f1 n (L.length tau);
             assert (truth_value_literal (pos_var_to_lit v1) tau = truth_value f1 tau);
-            //lemma_not_clauses v1 v tau
+            lemma_not_clauses v1 v tau;
             assert (truth_value_literal (pos_var_to_lit v) tau = truth_value (Not f1) tau)
       in
       forall_intro (move_requires aux)
 
 
-let prove_can_extend_not (f1:formula_t) (rf1 : list (list int)) (v1:int) (n:nat)
-                         (start_interval:nat) (end_interval:nat) (rf : list (list int)) (v:int)
-    : Lemma (requires n <= start_interval /\ start_interval <= v /\ v < end_interval /\
-                      valid f1 rf1 v1 n start_interval v /\
-                      tseitin_can_extend f1 rf1 v1 n start_interval v /\
-                      rf = L.append rf1 (not_clauses v1 v) /\ end_interval = v + 1)
-            (ensures valid (Not f1) rf v n start_interval end_interval /\
-                     tseitin_can_extend (Not f1) rf v n start_interval end_interval)
-    = assert (n <= v);
-      assert (valid (Not f1) rf v n start_interval end_interval);
-      let aux (tau : list bool) : Lemma (requires L.length tau = n)
-                                        (ensures can_extend tau (Not f1) rf v n start_interval end_interval)
-          = assert (can_extend tau f1 rf1 v1 n start_interval v);
-            assert (valid_literal (pos_var_to_lit v1))
+// let prove_same_value_or (f1:formula_t) (rf1 : list (list int)) (v1:int)
+//                         (f2:formula_t) (rf2 : list (list int)) (v2:int)
+//                         (n:nat) (start_interval:nat) (mid:nat) (end_interval:nat)
+//                         (v:int) (rf : list (list int))
+//     : Lemma (requires n <= start_interval /\ start_interval <= mid /\ mid <= v /\
+//                       valid f1 rf1 v1 n start_interval mid /\
+//                       tseitin_same_value f1 rf1 v1 n start_interval mid /\
+//                       valid f2 rf2 v2 n mid v /\
+//                       tseitin_same_value f2 rf2 v2 n mid v /\
+//                       rf = rf1 @ rf2 @ (or_clauses v1 v2 v) /\
+//                       end_interval = v + 1)
+//             (ensures valid (Or f1 f2) rf v n start_interval end_interval /\
+//                      tseitin_same_value (Or f1 f2) rf v n start_interval end_interval)
+//     = LP.append_assoc rf1 rf2 (or_clauses v1 v2 v);
+//       append_valid_cnf_formulas rf1 rf2;
+//       append_valid_cnf_formulas (rf1 @ rf2) (or_clauses v1 v2 v);
+//       // assert (variables_in_interval rf n start_interval end_interval);
+//       // assert (valid (Or f1 f2) rf v n start_interval end_interval);
 
-// lemma proveCanExtendNot(f1 : FormulaT, rf1 : seq<seq<int>>, v1 : int,
-//         n : int, start : int, v : int,
-//         end : int, rf : seq<seq<int>>)
-//         requires 0 <= n <= start <= v < end;
-//         requires valid(f1, rf1, v1, n, start, v);
-//         requires tseitinCanExtend(f1, rf1, v1, n, start, v);
-//         requires rf == rf1 + notClauses(v1, v);
-//         requires end == v + 1;
-//         ensures valid(Not(f1), rf, v, n, start, end);
-//         ensures tseitinCanExtend(Not(f1), rf, v, n, start, end);
-//     {
-//         assert 0 <= n <= v;
-//         assert valid(Not(f1), rf, v, n, start, end);
-//         forall tau : seq<bool> | |tau| == n
-//             ensures canExtend(tau, Not(f1), rf, v, n, start, end);
-//         {
-//             assert canExtend(tau, f1, rf1, v1, n, start, v);
-//             assert validLiteral(posVarToLit(v1));
+//       let aux (tau : list bool) 
+//           : Lemma (requires L.length tau >= end_interval /\
+//                             truth_value_cnf_formula rf tau)
+//                   (ensures truth_value_literal (pos_var_to_lit v) tau = truth_value (Or f1 f2) tau)
+//           = assert (variables_up_to_cnf_formula rf (L.length tau));
+//             variables_up_to_monotone f1 n (L.length tau);
+//             variables_up_to_monotone f2 n (L.length tau);
+//             assert (truth_value_literal (pos_var_to_lit v1) tau = truth_value f1 tau);
+//             assert (truth_value_literal (pos_var_to_lit v2) tau = truth_value f2 tau);
+//             lemma_or_clauses v1 v2 v tau;
+//             assert (truth_value_literal (pos_var_to_lit v) tau = truth_value (Or f1 f2) tau)
+//       in
+//       forall_intro (move_requires aux)
 
-//             ghost var tau1 :|
-//                 tau <= tau1 &&
-//                 |tau1| == v &&
-//                 truthValueCnfFormula(rf1, tau1) &&
-//                 truthValue(f1, tau) ==
-//                 truthValueLiteral(posVarToLit(v1), tau1);
 
-//             negateLiteral(v1, tau1);
+// let prove_same_value_and (f1:formula_t) (rf1 : list (list int)) (v1:int)
+//                          (f2:formula_t) (rf2 : list (list int)) (v2:int)
+//                          (n:nat) (start_interval:nat) (mid:nat) (end_interval:nat)
+//                          (v:int) (rf : list (list int))
+//     : Lemma (requires n <= start_interval /\ start_interval <= mid /\ mid <= v /\
+//                       valid f1 rf1 v1 n start_interval mid /\
+//                       tseitin_same_value f1 rf1 v1 n start_interval mid /\
+//                       valid f2 rf2 v2 n mid v /\
+//                       tseitin_same_value f2 rf2 v2 n mid v /\
+//                       rf = rf1 @ rf2 @ (and_clauses v1 v2 v) /\
+//                       end_interval = v + 1)
+//             (ensures valid (And f1 f2) rf v n start_interval end_interval /\
+//                      tseitin_same_value (And f1 f2) rf v n start_interval end_interval)
+//     = LP.append_assoc rf1 rf2 (and_clauses v1 v2 v);
+//       append_valid_cnf_formulas rf1 rf2;
+//       append_valid_cnf_formulas (rf1 @ rf2) (and_clauses v1 v2 v);
+//       // assert (variables_in_interval rf n start_interval end_interval);
+//       // assert (valid (And f1 f2) rf v n start_interval end_interval);
 
-//             ghost var tau' := combine1(tau, tau1, n, start, v,
-//                 truthValue(Not(f1), tau));
+//       let aux (tau : list bool) 
+//           : Lemma (requires L.length tau >= end_interval /\
+//                             truth_value_cnf_formula rf tau)
+//                   (ensures truth_value_literal (pos_var_to_lit v) tau = truth_value (And f1 f2) tau)
+//           = assert (variables_up_to_cnf_formula rf (L.length tau));
+//             variables_up_to_monotone f1 n (L.length tau);
+//             variables_up_to_monotone f2 n (L.length tau);
+//             assert (truth_value_literal (pos_var_to_lit v1) tau = truth_value f1 tau);
+//             assert (truth_value_literal (pos_var_to_lit v2) tau = truth_value f2 tau);
+//             lemma_and_clauses v1 v2 v tau;
+//             assert (truth_value_literal (pos_var_to_lit v) tau = truth_value (And f1 f2) tau)
+//       in
+//       forall_intro (move_requires aux)
 
-//             assert tau <= tau';
-//             assert |tau'| == end;
-//             transferTruthValue(rf1, tau1, tau', n, start, v);
 
-//             transferTruthValueLit(posVarToLit(v1), tau1, tau', n, start, v);
-//             assert truthValueLiteral(posVarToLit(v1), tau') ==
-//                 truthValue(f1, tau);
-//             transferTruthValueLit(negVarToLit(v1), tau1, tau', n, start, v);
-//             assert truthValueLiteral(negVarToLit(v1), tau1) ==
-//                 !truthValueLiteral(posVarToLit(v1), tau1);
+// let prove_same_value_implies (f1:formula_t) (rf1 : list (list int)) (v1:int)
+//                              (f2:formula_t) (rf2 : list (list int)) (v2:int)
+//                              (n:nat) (start_interval:nat) (mid:nat) (end_interval:nat)
+//                              (v:int) (rf : list (list int))
+//     : Lemma (requires n <= start_interval /\ start_interval <= mid /\ mid <= v /\
+//                       valid f1 rf1 v1 n start_interval mid /\
+//                       tseitin_same_value f1 rf1 v1 n start_interval mid /\
+//                       valid f2 rf2 v2 n mid v /\
+//                       tseitin_same_value f2 rf2 v2 n mid v /\
+//                       rf = rf1 @ rf2 @ (implies_clauses v1 v2 v) /\
+//                       end_interval = v + 1)
+//             (ensures valid (Implies f1 f2) rf v n start_interval end_interval /\
+//                      tseitin_same_value (Implies f1 f2) rf v n start_interval end_interval)
+//     = LP.append_assoc rf1 rf2 (implies_clauses v1 v2 v);
+//       append_valid_cnf_formulas rf1 rf2;
+//       append_valid_cnf_formulas (rf1 @ rf2) (implies_clauses v1 v2 v);
+//       // assert (variables_in_interval rf n start_interval end_interval);
+//       // assert (valid (Implies f1 f2) rf v n start_interval end_interval);
 
-//             lemmaNotClauses(v1, v, tau');
+//       let aux (tau : list bool) 
+//           : Lemma (requires L.length tau >= end_interval /\
+//                             truth_value_cnf_formula rf tau)
+//                   (ensures truth_value_literal (pos_var_to_lit v) tau = truth_value (Implies f1 f2) tau)
+//           = assert (variables_up_to_cnf_formula rf (L.length tau));
+//             variables_up_to_monotone f1 n (L.length tau);
+//             variables_up_to_monotone f2 n (L.length tau);
+//             assert (truth_value_literal (pos_var_to_lit v1) tau = truth_value f1 tau);
+//             assert (truth_value_literal (pos_var_to_lit v2) tau = truth_value f2 tau);
+//             lemma_and_clauses v1 v2 v tau;
+//             assert (truth_value_literal (pos_var_to_lit v) tau = truth_value (Implies f1 f2) tau)
+//       in
+//       forall_intro (move_requires aux)
 
-//             assert truthValueCnfFormula(rf, tau');
-//         }
-//     }
+
+// let prove_same_value_dimplies (f1:formula_t) (rf1 : list (list int)) (v1:int)
+//                               (f2:formula_t) (rf2 : list (list int)) (v2:int)
+//                               (n:nat) (start_interval:nat) (mid:nat) (end_interval:nat)
+//                               (v:int) (rf : list (list int))
+//     : Lemma (requires n <= start_interval /\ start_interval <= mid /\ mid <= v /\
+//                       valid f1 rf1 v1 n start_interval mid /\
+//                       tseitin_same_value f1 rf1 v1 n start_interval mid /\
+//                       valid f2 rf2 v2 n mid v /\
+//                       tseitin_same_value f2 rf2 v2 n mid v /\
+//                       rf = rf1 @ rf2 @ (dimplies_clauses v1 v2 v) /\
+//                       end_interval = v + 1)
+//             (ensures valid (DImplies f1 f2) rf v n start_interval end_interval /\
+//                      tseitin_same_value (DImplies f1 f2) rf v n start_interval end_interval)
+//     = LP.append_assoc rf1 rf2 (dimplies_clauses v1 v2 v);
+//       append_valid_cnf_formulas rf1 rf2;
+//       append_valid_cnf_formulas (rf1 @ rf2) (dimplies_clauses v1 v2 v);
+//       // assert (variables_in_interval rf n start_interval end_interval);
+//       // assert (valid (DImplies f1 f2) rf v n start_interval end_interval);
+
+//       let aux (tau : list bool) 
+//           : Lemma (requires L.length tau >= end_interval /\
+//                             truth_value_cnf_formula rf tau)
+//                   (ensures truth_value_literal (pos_var_to_lit v) tau = truth_value (DImplies f1 f2) tau)
+//           = assert (variables_up_to_cnf_formula rf (L.length tau));
+//             variables_up_to_monotone f1 n (L.length tau);
+//             variables_up_to_monotone f2 n (L.length tau);
+//             assert (truth_value_literal (pos_var_to_lit v1) tau = truth_value f1 tau);
+//             assert (truth_value_literal (pos_var_to_lit v2) tau = truth_value f2 tau);
+//             lemma_and_clauses v1 v2 v tau;
+//             assert (truth_value_literal (pos_var_to_lit v) tau = truth_value (DImplies f1 f2) tau)
+//       in
+//       forall_intro (move_requires aux)
+  
+  
+
+// let prove_can_extend_not (f1:formula_t) (rf1 : list (list int)) (v1:int) (n:nat)
+//                          (start_interval:nat) (end_interval:nat) (rf : list (list int)) (v:int)
+//     : Lemma (requires n <= start_interval /\ start_interval <= v /\ v < end_interval /\
+//                       valid f1 rf1 v1 n start_interval v /\
+//                       tseitin_can_extend f1 rf1 v1 n start_interval v /\
+//                       rf = L.append rf1 (not_clauses v1 v) /\ end_interval = v + 1)
+//             (ensures valid (Not f1) rf v n start_interval end_interval /\
+//                      tseitin_can_extend (Not f1) rf v n start_interval end_interval)
+//     = assert (n <= v);
+//       assert (valid (Not f1) rf v n start_interval end_interval);
+//       let aux (tau : list bool) : Lemma (requires L.length tau = n)
+//                                         (ensures can_extend tau (Not f1) rf v n start_interval end_interval)
+//           = assert (can_extend tau f1 rf1 v1 n start_interval v);
+//             assert (valid_literal (pos_var_to_lit v1));
+//             // let ghost tau1 : list bool = exists (tau1 : list bool) . L.length tau1 = v in
+//             // negate_literal v1 tau1
+//             // let (|tau1, _|) = exists (tau1 : list bool) . L.length tau1 = v in
+//             // negate_literal v1 tau1     
+//             let tau1 = exists_elim (exists (tau1 : list bool) . L.length tau1 = v) in
+//             negate_literal v1 tau1
+//       in
+//       forall_intro (move_requires aux) 
